derived_nat.thy
@@ -1,16 +1,23 @@
 theory derived_nat
   imports basic_definitions
-          derived_many
+          derived_many1
           derived_digit_char
 
           meta_digit_to_nat_and_back
 begin
 
+lemma digit_chars_eq_digit_chars[simp]:
+  "meta_digit_to_nat_and_back.digit_chars = derived_digit_char.digit_chars"
+  unfolding digit_chars_def
+  by blast
+
+
+
 definition nat_b :: "nat bidef" where
   "nat_b = transform
                    nat_from  \<comment> \<open>str \<Rightarrow> nat\<close>
                    print_nat  \<comment> \<open>nat \<Rightarrow> str\<close>
-                   (many digit_char)  \<comment> \<open>str bidef\<close>
+                   (many1 digit_char)  \<comment> \<open>str bidef\<close>
 "
 
 
@@ -31,7 +38,24 @@ lemma nat_is_nonterm[NER_simps]:
 
 lemma nat_is_error[NER_simps]:
   "is_error (parse nat_b) i \<longleftrightarrow> i = [] \<or> hd i \<notin> digit_chars"
+  unfolding nat_b_def
+  by (clarsimp simp add: NER_simps)
 
+lemma nat_has_result[NER_simps]:
+  "has_result (parse nat_b) i r l \<longleftrightarrow> i \<noteq> [] \<and> (\<exists> consumed . consumed \<noteq> [] \<and> i = consumed @ l \<and> r = (nat_from consumed) \<and> consumed = takeWhile (\<lambda>x. x\<in>digit_chars) i \<and> l = dropWhile (\<lambda>x. x\<in>digit_chars) i)"
+  unfolding nat_b_def
+  apply (auto simp add: NER_simps)
+  subgoal by (simp add: takeWhile_eq_Nil_iff)
+  subgoal
+          
+    sorry
+  subgoal
+    
+    sorry
+  subgoal by (metis \<open>\<And>r'. \<lbrakk>r' \<noteq> []; i \<noteq> []; hd r' = hd i; hd i \<in> derived_digit_char.digit_chars; has_result (parse (many digit_char)) (tl i) (tl r') l; r = nat_from r'\<rbrakk> \<Longrightarrow> i = takeWhile (\<lambda>x. x \<in> derived_digit_char.digit_chars) i @ l\<close> append_eq_conv_conj dropWhile_eq_drop)
+  subgoal
+    
+    sorry
 
 
 end
